\documentclass[parskip=full, draft]{scrartcl}
\input{~/Documents/Tripos/Solutions/examplesheet.tex}
\begin{document}
\addtitle{Definition of group}
\listoftodos
\begin{prob}{3}
    Prove that \((gh)^{-1} = h^{-1}g^{-1}\) for all elements \(g, h\) of a group \(G\).
\end{prob}
\begin{sol}
    We know that \(gh\) has an inverse, so it suffices to show that \(h^{-1}g^{-1}\) is a left inverse by uniqueness of inverse. We have
    \[
        h^{-1}g^{-1}gh = h^{-1}(g^{-1}g)h = h^{-1}eh = h^{-1} h = e.
    \]
\end{sol}
\end{document}