\lecture{2}{24 Jan. 10:00}{}
If we're in Cartesian, then we just differentiate vector components
\[\mathbf{x} (t) = x^i(t)\mathbf{e} _i \implies \dot{\mathbf{x}}(t) = \dot{\mathbf{x}}^i\mathbf{e}_{i}. \]
We also have the identities
\begin{align*}
    \frac{\mathrm{d}}{\mathrm{d}t} (\mathbf{f} \mathbf{g}) &= \dot{\mathbf{f} }g + f \dot{\mathbf{g} },\\
    \frac{\mathrm{d}}{\mathrm{d}t} (\mathbf{f} \mathbf{g}) &= \dot{\mathbf{f} }g + f \dot{\mathbf{g} },\\
    \frac{\mathrm{d}}{\mathrm{d}t} (\mathbf{f} \mathbf{g}) &= \dot{\mathbf{f} }g + f \dot{\mathbf{g} },
\end{align*}
which can be proved by applying the product rule to the component.